.vscode/Test.v
@@ -1,12 +1,11 @@
 From Ceres Require Import CeresParser.
 From Ceres Require Import Ceres.
 
-From Coq Require Import Ascii.
 From Coq Require Import List.
 Import ListNotations.
 
-From Coq Require Import String.
-Open Scope string_scope.
+From MetaRocq.Utils Require Import bytestring.
+Open Scope bs_scope.
 
 Definition exp : sexp := Atom_ (Str "hello world ∃ ? .- ၍").
 Definition s : string := string_of_sexp exp.
